Added key to crypto predicates along the usages

src/core/DY.Core.Bytes.fst
@@ -739,10 +739,10 @@ let has_kem_sk_usage #cusgs = mk_has_xxx_usage extract_kem_sk
 
 noeq
 type aead_crypto_predicate {|crypto_usages|} = {
-  pred: tr:trace -> key_usage:usage{AeadKey? key_usage} -> key:bytes -> nonce:bytes -> msg:bytes -> ad:bytes -> prop;
+  pred: tr:trace -> key_usage:usage{AeadKey? key_usage} -> key:bytes{key `has_usage tr` key_usage} -> nonce:bytes -> msg:bytes -> ad:bytes -> prop;
   pred_later:
     tr1:trace -> tr2:trace ->
-    key_usage:usage{AeadKey? key_usage} -> key:bytes -> nonce:bytes -> msg:bytes -> ad:bytes ->
+    key_usage:usage{AeadKey? key_usage} -> key:bytes{key `has_usage tr1` key_usage} -> nonce:bytes -> msg:bytes -> ad:bytes ->
     Lemma
     (requires
       pred tr1 key_usage key nonce msg ad /\
@@ -752,18 +752,22 @@ type aead_crypto_predicate {|crypto_usages|} = {
       bytes_well_formed tr1 ad /\
       tr1 <$ tr2
     )
-    (ensures pred tr2 key_usage key nonce msg ad)
+    (ensures 
+      key `has_usage tr2` key_usage /\
+      pred tr2 key_usage key nonce msg ad
+    )
   ;
 }
 
 noeq
 type pke_crypto_predicate {|crypto_usages|} = {
-  pred: tr:trace -> sk_usage:usage{PkeKey? sk_usage} -> pk:bytes -> msg:bytes -> prop;
+  pred: tr:trace -> sk_usage:usage{PkeKey? sk_usage} -> pk:bytes{pk `has_sk_usage tr` sk_usage} -> msg:bytes -> prop;
   pred_later:
     tr1:trace -> tr2:trace ->
     sk_usage:usage{PkeKey? sk_usage} -> pk:bytes -> msg:bytes ->
     Lemma
     (requires
+      pk `has_sk_usage tr1` sk_usage /\
       pred tr1 sk_usage pk msg /\
       bytes_well_formed tr1 pk /\
       bytes_well_formed tr1 msg /\
@@ -775,12 +779,13 @@ type pke_crypto_predicate {|crypto_usages|} = {
 
 noeq
 type sign_crypto_predicate {|crypto_usages|} = {
-  pred: tr:trace -> sk_usage:usage{SigKey? sk_usage} -> vk:bytes -> msg:bytes -> prop;
+  pred: tr:trace -> sk_usage:usage{SigKey? sk_usage} -> vk:bytes{vk `has_signkey_usage tr` sk_usage} -> msg:bytes -> prop;
   pred_later:
     tr1:trace -> tr2:trace ->
     sk_usage:usage{SigKey? sk_usage} -> vk:bytes -> msg:bytes ->
     Lemma
     (requires
+      vk `has_signkey_usage tr1` sk_usage /\
       pred tr1 sk_usage vk msg /\
       bytes_well_formed tr1 vk /\
       bytes_well_formed tr1 msg /\
@@ -964,7 +969,7 @@ let rec bytes_invariant #cinvs tr b =
         exists sk_usg.
         // Honest case:
         // - the key has the usage of signature key
-        sk `has_usage tr` sk_usg /\
+        (Vk sk) `has_signkey_usage tr` sk_usg /\
         SigKey? sk_usg /\
         // - the custom (protocol-specific) invariant hold (authentication)
         sign_pred.pred tr sk_usg (Vk sk) msg /\
@@ -1121,9 +1126,16 @@ let rec bytes_invariant_later #cinvs tr1 tr2 msg =
     bytes_invariant_later tr1 tr2 nonce;
     bytes_invariant_later tr1 tr2 msg;
     bytes_invariant_later tr1 tr2 ad;
-    introduce forall key_usg. aead_pred.pred tr1 key_usg key nonce msg ad ==> aead_pred.pred tr2 key_usg key nonce msg ad with (
-      introduce aead_pred.pred tr1 key_usg key nonce msg ad ==> aead_pred.pred tr2 key_usg key nonce msg ad with _. (
-        aead_pred.pred_later tr1 tr2 key_usg key nonce msg ad
+    introduce (exists key_usg. key `has_usage tr1` key_usg /\ AeadKey? key_usg /\ aead_pred.pred tr1 key_usg key nonce msg ad) ==> 
+      (exists key_usg. key `has_usage tr2` key_usg /\ aead_pred.pred tr2 key_usg key nonce msg ad)
+    with _. (
+      assert(exists key_usg. key `has_usage tr1` key_usg /\ AeadKey? key_usg /\ aead_pred.pred tr1 key_usg key nonce msg ad);
+      eliminate exists key_usg. key `has_usage tr1` key_usg /\ AeadKey? key_usg /\ aead_pred.pred tr1 key_usg key nonce msg ad
+      returns (exists key_usg. key `has_usage tr2` key_usg /\ aead_pred.pred tr2 key_usg key nonce msg ad)
+      with _. (
+        aead_pred.pred_later tr1 tr2 key_usg key nonce msg ad;
+        assert(exists key_usg. key `has_usage tr2` key_usg /\ aead_pred.pred tr2 key_usg key nonce msg ad);
+        ()
       )
     )
   )
@@ -1133,7 +1145,18 @@ let rec bytes_invariant_later #cinvs tr1 tr2 msg =
     bytes_invariant_later tr1 tr2 pk;
     bytes_invariant_later tr1 tr2 nonce;
     bytes_invariant_later tr1 tr2 msg;
-    FStar.Classical.forall_intro_3 (FStar.Classical.move_requires_3 (pke_pred.pred_later tr1 tr2))
+    introduce (exists sk_usg. pk `has_sk_usage tr1` sk_usg /\ PkeKey? sk_usg /\ pke_pred.pred tr1 sk_usg pk msg) ==>
+      (exists sk_usg. pk `has_sk_usage tr2` sk_usg /\ pke_pred.pred tr2 sk_usg pk msg)
+    with _. (
+      assert(exists sk_usg. pk `has_sk_usage tr1` sk_usg /\ PkeKey? sk_usg /\ pke_pred.pred tr1 sk_usg pk msg);
+      eliminate exists sk_usg. pk `has_sk_usage tr1` sk_usg /\ PkeKey? sk_usg /\ pke_pred.pred tr1 sk_usg pk msg
+      returns (exists sk_usg. pk `has_sk_usage tr2` sk_usg /\ pke_pred.pred tr2 sk_usg pk msg)
+      with _. (
+        pke_pred.pred_later tr1 tr2 sk_usg pk msg;
+        assert(exists sk_usg. pk `has_sk_usage tr2` sk_usg /\ pke_pred.pred tr2 sk_usg pk msg);
+        ()
+      )
+    )
   )
   | Vk sk ->
     bytes_invariant_later tr1 tr2 sk
@@ -1142,7 +1165,19 @@ let rec bytes_invariant_later #cinvs tr1 tr2 msg =
     bytes_invariant_later tr1 tr2 nonce;
     bytes_invariant_later tr1 tr2 msg;
     assert(bytes_invariant tr1 (Vk sk)); // to prove well-formedness
-    FStar.Classical.forall_intro_3 (FStar.Classical.move_requires_3 (sign_pred.pred_later tr1 tr2))
+    let vk = Vk sk in
+    introduce (exists sk_usg. vk `has_signkey_usage tr1` sk_usg /\ SigKey? sk_usg /\ sign_pred.pred tr1 sk_usg vk msg) ==>
+      (exists sk_usg. vk `has_signkey_usage tr2` sk_usg /\ sign_pred.pred tr2 sk_usg vk msg)
+    with _. (
+      assert(exists sk_usg. vk `has_signkey_usage tr1` sk_usg /\ SigKey? sk_usg /\ sign_pred.pred tr1 sk_usg vk msg);
+      eliminate exists sk_usg. vk `has_signkey_usage tr1` sk_usg /\ SigKey? sk_usg /\ sign_pred.pred tr1 sk_usg vk msg
+      returns (exists sk_usg. vk `has_signkey_usage tr2` sk_usg /\ sign_pred.pred tr2 sk_usg vk msg)
+      with _. (
+        sign_pred.pred_later tr1 tr2 sk_usg vk msg;
+        assert(exists sk_usg. vk `has_signkey_usage tr2` sk_usg /\ sign_pred.pred tr2 sk_usg vk msg);
+        ()
+      )
+    )
   )
   | Hash msg ->
     bytes_invariant_later tr1 tr2 msg
@@ -2242,7 +2277,7 @@ let bytes_invariant_verify #cinvs tr vkey sk_usg msg signature =
   normalize_term_spec get_label;
   normalize_term_spec vk;
   FStar.Classical.forall_intro_3 (FStar.Classical.move_requires_3 (has_usage_inj tr));
-  assert(forall sk. Vk sk == vk sk)
+  assert(forall sk sk_usg. (Vk sk) `has_signkey_usage tr` sk_usg == (vk sk) `has_signkey_usage tr` sk_usg)
 
 (*** Hash ***)
 
